templates/flows/gmap_more.v
@@ -277,7 +277,7 @@ Proof.
   apply Hf.
 Qed.
 
-Instance pmap_positive_imerge : Imerge Pmap positive :=
+Global Instance pmap_positive_imerge : Imerge Pmap positive :=
   {|
     imerge A B C := Pimerge;
     imerge_prf A B C := Pimerge_prf
@@ -325,7 +325,7 @@ Proof.
   all: auto.
 Qed.
 
-Instance gmap_Imerge `{Countable K} : Imerge (gmap K) K :=
+Global Instance gmap_Imerge `{Countable K} : Imerge (gmap K) K :=
   {|
     imerge A B C := gmap_imerge;
     imerge_prf A B C := gmap_imerge_prf
