templates/flows/list_flow_upd_insert.v
@@ -598,6 +598,77 @@ Section list_flow_upd_insert.
         clear -Insets_S H''; set_solver.
   Qed.
 
+  Lemma list_flow_upd_insert_S_in_nk Key n R Nx Mk S I I' II' nk n0:
+    let FI := λ I x, I !!! x in 
+    (nx_key_rel Nx Key) →
+    (nx_mk_closed Nx Mk (dom I)) →
+    (✓ ([^op set] x ∈ dom I, FI I x)) →
+    (∀ x, x ∈ dom I → Mk !!! x = true → keyset (FI I x) = ∅) →
+    (∀ x, x ∈ dom I → Mk !!! x = false → 
+            Key !!! n0 < Key !!! x → S ## outsets (FI I x)) → 
+    (∀ n1 n2, Nx !! n1 = Some n2 → dom (out_map (FI I n1)) = {[n2]}) →
+    (∀ x, x ∈ dom I → dom (FI I x) = {[x]}) →
+    (n ∈ dom I') → (dom I' ⊆ dom I) →
+    (Key !!! n0 < Key !!! n) →
+    (S ⊆ insets (FI I n)) →
+    (∀ x, x ∈ dom I' → Key !!! x ≤ Key !!! n) →
+    list_flow_upd_rec f_decr n R Nx Mk S I I' = Some (II', nk) →
+      (S ⊆ keyset (FI I nk)).
+  Proof.
+    intros FI. apply list_flow_upd_rec_ind; try done; last first.
+    - clear n R Nx Mk S I I'.
+      intros n R Nx Mk S I I0 n_in_R Hmk_n.
+      intros Nx_key Hcl VI KS_mk Disj_outsets Nx_dom Domm_I n_in_I0 
+        Dom_I0_in_I Key_n0 Insets_S Key_I0 [= -> ->].
+      apply lookup_total_correct in Hmk_n.
+      pose proof Disj_outsets nk (Dom_I0_in_I nk n_in_I0) Hmk_n Key_n0 as H'.
+      clear -Insets_S H'; set_solver.
+    - clear n R Nx Mk S I I'.
+      intros n R Nx Mk S I I0 n_in_R Hmk_n n1 Hnx_n In In' In1 In1' II I0'.
+      intros HInd Nx_key Hcl VI KS_mk Disj_outsets Nx_dom Domm_I n_in_I0 
+        Dom_I0_in_I Key_n0 Insets_S Key_I0 Hflow.
+      assert (n1 ∉ dom I0) as n1_notin_I0.
+      { pose proof Nx_key n n1 Hnx_n as H'.
+        intros n1_in_I0. apply Key_I0 in n1_in_I0.
+        clear -H' n1_in_I0. lia. }
+      assert (dom I0' = dom I0 ∪ {[ n1 ]}) as Dom_I0'.
+      { rewrite /I0' /II. repeat rewrite dom_insert_L.
+        clear -n_in_I0 n1_notin_I0. set_solver. }
+      assert (n1 ∈ dom I) as n1_in_I.
+      { destruct Hcl as [_ [_ Hcl]].
+        by pose proof Hcl n n1 Hnx_n as H'. }
+      assert (S ⊆ outsets (FI I n)) as Outsets_S.
+      { apply lookup_total_correct in Hmk_n. apply KS_mk in Hmk_n.
+        rewrite /keyset in Hmk_n. clear -Hmk_n Insets_S.
+        assert (insets (FI I n) ⊆ outsets (FI I n)). set_solver. set_solver.
+        by apply Dom_I0_in_I in n_in_I0. } 
+      assert (S ⊆ insets (FI I n1)) as Insets_S'.
+      { intros k Hk. rewrite /insets Domm_I. rewrite big_opS_singleton.
+        apply Outsets_S in Hk. rewrite /outsets in Hk.
+        rewrite (Nx_dom n n1 Hnx_n) big_opS_singleton in Hk.
+        apply (flowint_inset_step (FI I n)); try done.
+        assert ({[n;n1]} ⊆ dom I) as H'.
+        { clear -n1_in_I n_in_I0 Dom_I0_in_I; set_solver. }
+        pose proof flow_big_op_valid _ _ _ H' VI  as H''.
+        rewrite (big_opS_delete _ _ n) in H''.
+        assert ({[n;n1]} ∖ {[n]} = ({[n1]}: gset Node)) as H1'.
+        { clear -n1_notin_I0 n_in_I0; set_solver. }
+        by rewrite H1' big_opS_singleton in H''.
+        clear; set_solver.
+        rewrite Domm_I. clear; set_solver.
+        done. done. }
+      apply HInd; try done; clear HInd.
+      + rewrite Dom_I0'; clear; set_solver.
+      + rewrite Dom_I0'; clear -Dom_I0_in_I n1_in_I; set_solver.
+      + pose proof Nx_key n n1 Hnx_n as H'. clear -Key_n0 H'; lia. 
+      + pose proof Nx_key n n1 Hnx_n as H'. 
+        rewrite Dom_I0'. intros x; rewrite elem_of_union.
+        intros [Hx | Hx].
+        * apply Key_I0 in Hx. clear -Hx H'. lia.
+        * assert (x = n1) as -> by (clear -Hx; set_solver).
+          clear; try done.
+  Qed.
+
   Lemma list_flow_upd_insert_KS_nk Key n R Nx Mk S I I' II' nk:
     let FI := λ I x, I !!! x in 
     (nx_key_rel Nx Key) →
@@ -629,7 +700,7 @@ Section list_flow_upd_insert.
         apply leibniz_equiv. rewrite !big_opS_singleton.
         rewrite inflow_delete_set_inset. done.
         intros k _; apply (Inf_x nk); try done. }
-      set_solver.
+      clear; set_solver.
     - clear n R Nx Mk S I I'.
       intros n R Nx Mk S I I0 n_in_R Hmk_n n1 Hnx_n In In' In1 In1' II I0'.
       intros HInd Nx_key Hcl VI KS_mk Nx_dom Domm_I Inf_x n_in_I0 Dom_I0_in_I 
@@ -919,13 +990,188 @@ Section list_flow_upd_insert.
           by rewrite /inflow_map_set /= /In1.  
   Qed.
 
+  Lemma list_flow_upd_insert_Out_In Key n R Nx Mk S I I' II' nk n0:
+    let FI := λ I x, I !!! x in 
+    (nx_key_rel Nx Key) →
+    (nx_mk_closed Nx Mk (dom I)) →
+    (∀ x, x ∈ dom I → Mk !!! x = true → keyset (FI I x) = ∅) →
+    (∀ x, x ∈ dom I → Mk !!! x = false → 
+            Key !!! n0 < Key !!! x → S ## outsets (FI I x)) → 
+    (✓ ([^op set] x ∈ dom I, FI I x)) →
+    (∀ n1 n2, Nx !! n1 = Some n2 → dom (out_map (FI I n1)) = {[n2]}) →
+    (∀ x, x ∈ dom I → dom (FI I x) = {[x]}) →
+    (∀ x, x ∈ dom I → outsets (FI I x) ⊆ insets (FI I x)) →
+    (∀ x k, x ∈ dom I → inf (FI I x) x !!! k ≤ 1) →
+    (∀ x x' k, x ∈ dom I → out (FI I x) x' !!! k ≤ 1) →
+    (n0 ∈ dom I') → (n ∈ dom I') → (n0 ≠ n) → (dom I' ⊆ dom I) →
+    (∀ x, x ∈ dom I' → Key !!! x ≤ Key !!! n) →
+    (∀ x, x ∈ dom I' ∖ {[n0]} → Key !!! n0 < Key !!! x) →
+    (FI I' n = inflow_map_set f_decr (FI I n) n S) →
+    (∃ k, k ∈ inset _ (FI I n) n ∧ k ∉ S) →
+    (∀ x, x ∈ dom I' ∖ {[n]} → outsets (FI I' x) ⊆ insets (FI I' x)) →
+    list_flow_upd_rec f_decr n R Nx Mk S I I' = Some (II', nk) →
+        (∀ x, x ∈ dom II' → outsets (FI II' x) ⊆ insets (FI II' x)).
+  Proof.
+    intros FI. apply list_flow_upd_rec_ind; try done; last first.
+    - clear n R Nx Mk S I I'.
+      intros n R Nx Mk S I I0 n_in_R Hmk_n.
+      intros Nx_key Hcl KS_mk Disj_outsets VI Nx_dom Domm_I Out_In Inf_x 
+        Out_x n0_in_I0 n_in_I0 n0_neq_n Dom_I0_in_I Key_I0 Key_n0 Def_I0_n 
+        Inset_k Out_In' [= -> ->].
+      intros x Hx. destruct (decide (x = nk)) as [-> | Hxnk]; last first.
+      { apply Out_In'. clear -Hx Hxnk; set_solver. }
+      rewrite Def_I0_n. rewrite inflow_delete_set_outsets.
+      assert (insets (inflow_map_set f_decr (FI I nk) nk S) = 
+        insets (FI I nk) ∖ S) as ->.
+      { rewrite /insets flowint_inflow_map_set_dom Domm_I. 
+        assert ({[nk; nk]} = {[nk]}) as -> by (clear; set_solver).
+        rewrite -leibniz_equiv_iff !big_opS_singleton.
+        rewrite inflow_delete_set_inset; try done.
+        intros k Hk. apply Inf_x. all: by apply Dom_I0_in_I. }
+      apply lookup_total_correct in Hmk_n.
+      assert (nk ∈ dom II' ∖ {[n0]}) as H'%Key_n0.
+      { clear -Hx n0_neq_n; set_solver. }
+      pose proof Disj_outsets nk (Dom_I0_in_I nk Hx) Hmk_n H' as H''.
+      pose proof Out_In nk (Dom_I0_in_I nk Hx) as H1'.
+      clear -H'' H1'; set_solver.
+    - clear n R Nx Mk S I I'.
+      intros n R Nx Mk S I I0 n_in_R Hmk_n n1 Hnx_n In In' In1 In1' II I0'.
+      intros HInd Nx_key Hcl KS_mk Disj_outsets VI Nx_dom Domm_I Out_In Inf_x 
+        Out_x n0_in_I0 n_in_I0 n0_neq_n Dom_I0_in_I Key_I0 Key_n0 Def_I0_n 
+        Inset_k Out_In' Hflow.
+      assert (n1 ∉ dom I0) as n1_notin_I0.
+      { pose proof Nx_key n n1 Hnx_n as H'.
+        intros n1_in_I0. apply Key_I0 in n1_in_I0.
+        clear -H' n1_in_I0. lia. }
+      assert (dom I0' = dom I0 ∪ {[ n1 ]}) as Dom_I0'.
+      { rewrite /I0' /II. repeat rewrite dom_insert_L.
+        clear -n_in_I0 n1_notin_I0. set_solver. }
+      assert (n1 ∈ dom I) as n1_in_I.
+      { destruct Hcl as [_ [_ Hcl]].
+        by pose proof Hcl n n1 Hnx_n as H'. }
+      assert (n ≠ n1) as n_neq_n1.
+      { clear -n_in_I0 n1_notin_I0. set_solver. }
+      assert (∃ k, k ∈ outset _ (FI I0 n) n1 ∧ k ∉ S) as Outset_k.
+      { destruct Inset_k as [k [H1' H1'']].
+        exists k. split; try done.
+        rewrite Def_I0_n. unfold outset.
+        rewrite nzmap_elem_of_dom_total.
+        unfold inflow_delete_set, inflow_map_set.
+        unfold out, out_map at 1. simpl.
+        assert (k ∈ outset _ (FI I n) n1) as H'.
+        { apply Dom_I0_in_I in n_in_I0.
+          apply lookup_total_correct in Hmk_n.
+          pose proof KS_mk n n_in_I0 Hmk_n as H'.
+          rewrite /keyset /FI in H'.
+          rewrite /insets /outsets (Domm_I n n_in_I0) 
+            (Nx_dom n n1 Hnx_n) in H'.
+          apply leibniz_equiv_iff in H'.
+          rewrite !big_opS_singleton in H'.
+          clear -H' H1'. set_solver. }
+        unfold outset in H'.
+        rewrite nzmap_elem_of_dom_total in H'.
+        by unfold out in H'. }
+      apply HInd; clear HInd; try done.
+      + rewrite Dom_I0'; clear -n0_in_I0; set_solver.
+      + rewrite Dom_I0'; clear; set_solver.
+      + clear -n0_in_I0 n1_notin_I0; set_solver.
+      + rewrite Dom_I0'; clear -Dom_I0_in_I n1_in_I; set_solver. 
+      + pose proof Nx_key n n1 Hnx_n as H'. 
+        rewrite Dom_I0'. intros x; rewrite elem_of_union.
+        intros [Hx | Hx].
+        * apply Key_I0 in Hx. clear -Hx H'. lia.
+        * assert (x = n1) as -> by (clear -Hx; set_solver).
+          clear; try done.
+      + rewrite Dom_I0'. intros x. rewrite elem_of_difference.
+        rewrite elem_of_union. intros [[Hx1 | Hx1] Hx2].
+        * apply Key_n0. clear -Hx1 Hx2; set_solver.
+        * assert (x = n1) as -> by (clear -Hx1; set_solver). 
+          pose proof Nx_key n n1 Hnx_n as H'.
+          assert (Key !!! n0 ≤ Key !!! n) as H''.
+          { by apply Key_I0. }
+          clear -H' H''. lia.
+      + by rewrite /I0' /FI lookup_total_insert /In1' /In1.
+      + destruct Inset_k as [k [H1' H1'']].
+        exists k. split; try done.
+        rewrite /FI /I0'. 
+        apply (flowint_inset_step (FI I n) (FI I n1) k n1); try done.
+        { assert ({[n; n1]} ⊆ dom I) as Hsub.
+          { clear -n1_in_I n_in_I0 Dom_I0_in_I. set_solver. }
+          pose proof (flow_big_op_valid _ _ {[n; n1]} Hsub VI) as VI'.
+          rewrite big_opS_union in VI'.
+          rewrite !big_opS_singleton in VI'.
+          by unfold FI in VI'. clear -n1_notin_I0 n_in_I0. set_solver. }
+        rewrite Domm_I. clear; set_solver. done.
+        apply Dom_I0_in_I in n_in_I0.
+        apply lookup_total_correct in Hmk_n.
+        pose proof KS_mk n n_in_I0 Hmk_n as H'.
+        rewrite /keyset /FI in H'.
+        rewrite /insets /outsets (Domm_I n n_in_I0) 
+          (Nx_dom n n1 Hnx_n) in H'.
+        apply leibniz_equiv_iff in H'.
+        rewrite !big_opS_singleton in H'.
+        clear -H' H1'. set_solver. 
+      + rewrite Dom_I0'. intros x; rewrite elem_of_difference elem_of_union.
+        intros [[Hx | Hx] Hxn1]; last first.
+        { clear -Hx Hxn1; set_solver. }
+        destruct (decide (x = n)) as [-> | Hxn]; last first.
+        { rewrite /I0' /FI !lookup_total_insert_ne; try done.
+          apply Out_In'; try done. clear -n1_notin_I0 Hx Hxn; set_solver.
+          clear -Hx n1_notin_I0. set_solver. }
+        rewrite /I0' /FI lookup_total_insert_ne /II; try done.
+        rewrite lookup_total_insert /In' /In outflow_delete_set_insets.
+        assert (outsets (outflow_map_set f_decr (I0 !!! n) n1 S) = 
+          outsets (FI I0 n) ∖ S) as ->.
+        { rewrite {1}/outsets. 
+          set D := dom (out_map (outflow_map_set f_decr (I0 !!! n) n1 S)).
+          pose proof flowint_outflow_map_set_dom f_decr (I0 !!! n) n1 S as H'.
+          assert (dom (out_map (FI I0 n)) = {[n1]}) as Hdom.
+          { by rewrite Def_I0_n /inflow_map_set /= (Nx_dom n n1 Hnx_n). }
+          rewrite Hdom in H'. 
+          assert (D = ∅ ∨ D = {[n1]}) as HD.
+          { rewrite -/D in H'. clear -H'. 
+            assert ({[n1; n1]} = ({[n1]}: gset Node)) as H''.
+            clear; set_solver. rewrite H'' in H'.
+            destruct (decide (n1 ∈ D)); try set_solver. }
+          destruct HD as [HD | HD]; rewrite HD.
+          { rewrite /D /outflow_map_set /= in HD.
+            rewrite -leibniz_equiv_iff nzmap_dom_insert_nonzero in HD.
+            rewrite Hdom in HD. clear -HD; set_solver.
+            destruct Outset_k as [k [H1' H1'']].
+            clear H'. intros H'; rewrite nzmap_eq in H'.
+            pose proof H' k as H'. 
+            rewrite nzmap_lookup_total_map_set_ne in H'; try done.
+            rewrite /outset nzmap_elem_of_dom_total /ccmunit /= in H1'.
+            rewrite /ccmunit /= /lift_unit nzmap_lookup_empty /ccmunit /= in H'.
+            clear -H1' H'; try done. }
+          rewrite -leibniz_equiv_iff big_opS_singleton.
+          rewrite outflow_delete_set_outset /outsets. 
+          rewrite Hdom big_opS_singleton; try done.
+          rewrite /FI in Def_I0_n. rewrite Def_I0_n.
+          rewrite /inflow_map_set /out /=. rewrite /out /FI in Out_x. 
+          intros k Hk; apply Out_x. by apply Dom_I0_in_I. }
+        rewrite !Def_I0_n inflow_delete_set_outsets.
+        assert (insets (I0 !!! n) = insets (FI I n) ∖ S) as ->.
+        { rewrite /FI in Def_I0_n. rewrite Def_I0_n /insets.
+          rewrite flowint_inflow_map_set_dom Domm_I.
+          assert ({[n;n]} = {[n]}) as -> by (clear; set_solver).
+          rewrite -leibniz_equiv_iff !big_opS_singleton.
+          rewrite inflow_delete_set_inset; try done.
+          intros k Hk; apply Inf_x. all: by apply Dom_I0_in_I. }
+        pose proof Out_In n (Dom_I0_in_I n n_in_I0) as H'.
+        clear -H'; set_solver.
+  Qed.
+
     
   Lemma insert_flow_updk_summary Key n0 Nx Mk S I res n1:
     let FI := λ I x, I !!! x in 
     (nx_key_rel Nx Key) →
     (nx_mk_closed Nx Mk (dom I)) →
     (∀ x, x ∈ dom I → Mk !!! x = true → keyset (FI I x) = ∅) →
+    (∀ x, x ∈ dom I → Mk !!! x = false → 
+            Key !!! n0 < Key !!! x → S ## outsets (FI I x)) → 
     (∀ n1 n2, Nx !! n1 = Some n2 → dom (out_map (FI I n1)) = {[n2]}) →
+    (∀ x, x ∈ dom I → outsets (FI I x) ⊆ insets (FI I x)) →
     (Nx !! n0 = Some n1) →
     (✓ ([^op set] x ∈ dom I, FI I x)) →
     (∀ x, x ∈ dom I → dom (FI I x) = {[x]}) →
@@ -940,8 +1186,11 @@ Section list_flow_upd_insert.
       ∧ (dom II ⊆ dom I)
       ∧ (n0 ∈ dom II)
       ∧ (nk ∈ dom II)
+      ∧ (n0 ≠ nk)
       ∧ (Mk !! nk = Some false)
+      ∧ (∀ x, x ∈ dom II ∖ {[n0;nk]} → Mk !! x = Some true)
       ∧ (∀ x, x ∈ dom II ∖ {[nk]} → Nx !! x ≠ None)
+      ∧ (∀ x, x ∈ dom II ∖ {[n0]} → Key !!! n0 < Key !!! x)
       ∧ (∀ x, x ∈ dom II → dom (FI II x) = {[x]})
       ∧ (([^op set] x ∈ dom II, FI I x) = ([^op set] x ∈ dom II, FI II x))
       ∧ (FI II n0 = outflow_delete_set (FI I n0) n1 S)
@@ -951,12 +1200,14 @@ Section list_flow_upd_insert.
       ∧ (∀ x k, x ∈ dom II → inf (FI II x) x !!! k ≤ 1)
       ∧ (∀ x x' k, x ∈ dom II → out (FI II x) x' !!! k ≤ 1)
       ∧ (∀ x, x ∈ dom II → dom (out_map (FI II x)) = dom (out_map (FI I x)))
+      ∧ (∀ x, x ∈ dom II → outsets (FI II x) ⊆ insets (FI II x))
       ∧ (keyset (FI II n0) = keyset (FI I n0) ∪ S)
       ∧ (keyset (FI II nk) = keyset (FI I nk) ∖ S)
-      ∧ (∀ x, x ∈ dom II ∖ {[ n0; nk ]} → keyset (FI II x) = keyset (FI I x)).
+      ∧ (∀ x, x ∈ dom II ∖ {[ n0; nk ]} → keyset (FI II x) = keyset (FI I x))
+      ∧ (S ⊆ keyset (FI I nk)).
   Proof.
-    intros FI Nx_key Hcl KS_Mk Nx_dom Hnx_n0 VI Domm_I n0_in_I 
-      Insets_S Outset_S Inf_x Out_x Hflow.
+    intros FI Nx_key Hcl KS_Mk Disj_insets Nx_dom Out_In Hnx_n0 VI Domm_I 
+      n0_in_I Insets_S Outset_S Inf_x Out_x Hflow.
     unfold list_flow_upd_insert, list_flow_upd in Hflow.
     rewrite Hnx_n0 in Hflow. 
     set In1 := inflow_delete_set (I !!! n1) n1 S.
@@ -983,7 +1234,7 @@ Section list_flow_upd_insert.
         by set_solver. }
       clear -H' H''; set_solver. }  
     assert ((dom I ∖ {[n0]}) ∩ dom I' = {[n1]}) as H''.
-    { rewrite Dom_I'. set_solver. }
+    { rewrite Dom_I'. clear -n0_neq_n1 n1_in_I; set_solver. }
     assert (Key !!! n0 < Key !!! n1) as Key_n0_n1.
     { by apply Nx_key in Hnx_n0. }
     assert (∀ x : Node, x ∈ dom I' → Key !!! x ≤ Key !!! n1) as Key_I'.
@@ -1180,6 +1431,18 @@ Section list_flow_upd_insert.
       - rewrite /I' /FI lookup_total_insert_ne; try done.
         rewrite lookup_total_insert /In0. done.
       - by rewrite /I' /FI lookup_total_insert /In1 /inflow_map_set /=. }
+    assert (∀ x, x ∈ dom I' ∖ {[n1]} → 
+                  outsets (FI I' x) ⊆ insets (FI I' x)) as Out_In'.
+    { intros x. rewrite Dom_I' elem_of_difference elem_of_union.
+      intros [[Hx | Hx] Hx']; last first.
+      { clear -Hx Hx'; set_solver. }
+      rewrite elem_of_singleton in Hx; subst x.
+      rewrite /I' /FI lookup_total_insert_ne; try done.
+      rewrite lookup_total_insert H1'' /In0 outflow_delete_set_insets.
+      pose proof Out_In n0 n0_in_I as H'. clear -H'; set_solver. }
+    assert (∀ x, x ∈ dom I' ∖ {[n0; n1]} → Mk !! x = Some true) as Mk_x.
+    { intros x Hx; rewrite Dom_I' in Hx. clear -Hx; set_solver. }
+
     
     set R := dom I ∖ {[n0]}.
     
@@ -1187,8 +1450,11 @@ Section list_flow_upd_insert.
     - by apply (list_flow_upd_dom Key f_decr n1 R Nx Mk S I I' II nk).
     - by apply (list_flow_upd_n0_dom f_decr n1 R Nx Mk S I I' II nk).
     - by apply (list_flow_upd_nk_dom f_decr n1 R Nx Mk S I I' II nk).
+    - by apply (list_flow_upd_neq Key f_decr n1 R Nx Mk S I I' II nk). 
     - by apply (list_flow_upd_Mk_nk f_decr n1 R Nx Mk S I I' II nk).
+    - by apply (list_flow_upd_Mk f_decr n1 R Nx Mk S I I' II nk).
     - by apply (list_flow_upd_Nx Key f_decr n1 R Nx Mk S I I' II nk n0).
+    - by apply (list_flow_upd_Key_n0 Key f_decr n1 R Nx Mk S I I' II nk n0).
     - by apply (list_flow_upd_domm Key f_decr n1 R Nx Mk S I I' II nk).
     - by apply (list_flow_upd_insert_intfEq Key n1 R Nx Mk S I I' II nk n0).
     - by apply (list_flow_upd_II'_n0 Key f_decr n1 R Nx Mk S I I' II nk n0).
@@ -1197,11 +1463,13 @@ Section list_flow_upd_insert.
     - by apply (list_flow_upd_insert_Inf Key n1 R Nx Mk S I I' II nk).
     - by apply (list_flow_upd_insert_Out Key n1 R Nx Mk S I I' II nk).
     - by apply (list_flow_upd_insert_Dom_out Key n1 R Nx Mk S I I' II nk).
+    - by apply (list_flow_upd_insert_Out_In Key n1 R Nx Mk S I I' II nk n0).
     - rewrite /FI 
         (list_flow_upd_II'_n0 Key f_decr n1 R Nx Mk S I I' II nk n0 In0); 
         try done.
     - by apply (list_flow_upd_insert_KS_nk Key n1 R Nx Mk S I I' II nk).
     - by apply (list_flow_upd_insert_KS Key n1 R Nx Mk S I I' II nk n0).
+    - by apply (list_flow_upd_insert_S_in_nk Key n1 R Nx Mk S I I' II nk n0).
   Qed.
 
 End list_flow_upd_insert.
